theories/TransformerLens/HookedTransformer/Instances.v
@@ -27,8 +27,10 @@ Module HookedTransformer.
   Ltac t_step :=
     first [ match goal with
             | [ |- ?x = ?x ] => reflexivity
-            | [ |- ?R (PArray.checkpoint _ _) (PArray.checkpoint _ _) ]
-              => apply Tensor.PArray.checkpoint_Proper_dep
+            | [ |- ?R (PArray.checkpoint _ _) _ ]
+              => rewrite PArray.checkpoint_correct
+            | [ |- ?R _ (PArray.checkpoint _ _) ]
+              => rewrite PArray.checkpoint_correct
             | [ |- ?R (Tensor.of_bool _ _) (Tensor.of_bool _ _) ]
               => apply (Tensor.of_bool_Proper_dep _ _ R)
             | [ |- ?R (Tensor.map2 _ _ _ _) (Tensor.map2 _ _ _ _) ]
@@ -256,10 +258,13 @@ Module HookedTransformer.
              ==> (Dependent.idR ==> Dependent.idR)
              ==> Dependent.idR
              ==> (Dependent.const eq ==> Dependent.idR)
+             ==> Dependent.const (fun _ _ => True)
              ==> Dependent.idR
              ==> Tensor.eqfR ==> Tensor.eqfR ==> Tensor.eqfR ==> Tensor.eqfR)
           (@forward r s d_model).
-    Proof. cbv [forward]; t. Qed.
+    Proof. cbv [forward]; t.
+
+    Qed.
   End LayerNorm.
   Export (hints) LayerNorm.
 
@@ -285,6 +290,7 @@ Module HookedTransformer.
              ==> (Dependent.idR ==> Dependent.idR ==> Dependent.idR)
              ==> Dependent.idR
              ==> (Dependent.idR ==> Dependent.idR ==> Dependent.idR)
+             ==> Dependent.const (fun _ _ => True)
              ==> Tensor.eqfR
              ==> Tensor.eqfR
              ==> Tensor.eqfR
@@ -292,8 +298,8 @@ Module HookedTransformer.
           (@q r batch pos n_heads d_model d_head use_split_qkv_input).
     Proof. cbv [q]; repeat first [ t_step | apply einsum_input_Proper_dep ]. Qed.
 
-    #[export] Instance q_Proper {A r batch pos n_heads d_model d_head use_split_qkv_input coerZ addA zeroA mulA W_Q b_Q}
-      : Proper (Tensor.eqf ==> Tensor.eqf) (@q A r batch pos n_heads d_model d_head use_split_qkv_input coerZ addA zeroA mulA W_Q b_Q).
+    #[export] Instance q_Proper {A r batch pos n_heads d_model d_head use_split_qkv_input coerZ addA zeroA mulA use_checkpoint W_Q b_Q}
+      : Proper (Tensor.eqf ==> Tensor.eqf) (@q A r batch pos n_heads d_model d_head use_split_qkv_input coerZ addA zeroA mulA use_checkpoint W_Q b_Q).
     Proof. apply q_Proper_dep; repeat intro; subst; reflexivity. Qed.
 
     #[export] Instance k_Proper_dep {r batch pos n_heads d_model d_head use_split_qkv_input}
@@ -302,6 +308,7 @@ Module HookedTransformer.
              ==> (Dependent.idR ==> Dependent.idR ==> Dependent.idR)
              ==> Dependent.idR
              ==> (Dependent.idR ==> Dependent.idR ==> Dependent.idR)
+             ==> Dependent.const (fun _ _ => True)
              ==> Tensor.eqfR
              ==> Tensor.eqfR
              ==> Tensor.eqfR
@@ -309,8 +316,8 @@ Module HookedTransformer.
           (@k r batch pos n_heads d_model d_head use_split_qkv_input).
     Proof. cbv [k]; repeat first [ t_step | apply einsum_input_Proper_dep ]. Qed.
 
-    #[export] Instance k_Proper {A r batch pos n_heads d_model d_head use_split_qkv_input coerZ addA zeroA mulA W_K b_K}
-      : Proper (Tensor.eqf ==> Tensor.eqf) (@k A r batch pos n_heads d_model d_head use_split_qkv_input coerZ addA zeroA mulA W_K b_K).
+    #[export] Instance k_Proper {A r batch pos n_heads d_model d_head use_split_qkv_input coerZ addA zeroA mulA use_checkpoint W_K b_K}
+      : Proper (Tensor.eqf ==> Tensor.eqf) (@k A r batch pos n_heads d_model d_head use_split_qkv_input coerZ addA zeroA mulA use_checkpoint W_K b_K).
     Proof. apply k_Proper_dep; repeat intro; subst; reflexivity. Qed.
 
     #[export] Instance v_Proper_dep {r batch pos n_heads d_model d_head use_split_qkv_input}
@@ -319,6 +326,7 @@ Module HookedTransformer.
              ==> (Dependent.idR ==> Dependent.idR ==> Dependent.idR)
              ==> Dependent.idR
              ==> (Dependent.idR ==> Dependent.idR ==> Dependent.idR)
+             ==> Dependent.const (fun _ _ => True)
              ==> Tensor.eqfR
              ==> Tensor.eqfR
              ==> Tensor.eqfR
@@ -326,8 +334,8 @@ Module HookedTransformer.
           (@v r batch pos n_heads d_model d_head use_split_qkv_input).
     Proof. cbv [v]; repeat first [ t_step | apply einsum_input_Proper_dep ]. Qed.
 
-    #[export] Instance v_Proper {A r batch pos n_heads d_model d_head use_split_qkv_input coerZ addA zeroA mulA W_V b_V}
-      : Proper (Tensor.eqf ==> Tensor.eqf) (@v A r batch pos n_heads d_model d_head use_split_qkv_input coerZ addA zeroA mulA W_V b_V).
+    #[export] Instance v_Proper {A r batch pos n_heads d_model d_head use_split_qkv_input coerZ addA zeroA mulA use_checkpoint W_V b_V}
+      : Proper (Tensor.eqf ==> Tensor.eqf) (@v A r batch pos n_heads d_model d_head use_split_qkv_input coerZ addA zeroA mulA use_checkpoint W_V b_V).
     Proof. apply v_Proper_dep; repeat intro; subst; reflexivity. Qed.
 
     #[export] Instance attn_scores_Proper_dep {r batch pos n_heads d_model d_head use_split_qkv_input}
@@ -338,6 +346,7 @@ Module HookedTransformer.
              ==> Dependent.idR
              ==> (Dependent.idR ==> Dependent.idR ==> Dependent.idR)
              ==> (Dependent.idR ==> Dependent.idR ==> Dependent.idR)
+             ==> Dependent.const (fun _ _ => True)
              ==> Tensor.eqfR
              ==> Tensor.eqfR
              ==> Tensor.eqfR
@@ -346,10 +355,10 @@ Module HookedTransformer.
              ==> Tensor.eqfR
              ==> Tensor.eqfR)
           (@attn_scores r batch pos n_heads d_model d_head use_split_qkv_input).
-    Proof. cbv [attn_scores]; repeat first [ t_step | apply q_Proper_dep | apply k_Proper_dep ]. Qed.
+    Proof. cbv [attn_scores]; repeat first [ t_step | apply q_Proper_dep | apply k_Proper_dep | apply einsum_input_Proper_dep ]. Qed.
 
-    #[export] Instance attn_scores_Proper {r batch pos n_heads d_model d_head use_split_qkv_input A sqrtA coerZ addA zeroA mulA divA W_Q W_K b_Q b_K}
-      : Proper (Tensor.eqf ==> Tensor.eqf ==> Tensor.eqf) (@attn_scores r batch pos n_heads d_model d_head use_split_qkv_input A sqrtA coerZ addA zeroA mulA divA W_Q W_K b_Q b_K).
+    #[export] Instance attn_scores_Proper {r batch pos n_heads d_model d_head use_split_qkv_input A sqrtA coerZ addA zeroA mulA divA use_checkpoint W_Q W_K b_Q b_K}
+      : Proper (Tensor.eqf ==> Tensor.eqf ==> Tensor.eqf) (@attn_scores r batch pos n_heads d_model d_head use_split_qkv_input A sqrtA coerZ addA zeroA mulA divA use_checkpoint W_Q W_K b_Q b_K).
     Proof. apply attn_scores_Proper_dep; repeat intro; subst; reflexivity. Qed.
 
     #[export] Instance apply_causal_mask_Proper_dep {r batch pos n_heads n_ctx}
@@ -372,6 +381,7 @@ Module HookedTransformer.
              ==> Dependent.idR
              ==> (Dependent.idR ==> Dependent.idR ==> Dependent.idR)
              ==> (Dependent.idR ==> Dependent.idR ==> Dependent.idR)
+             ==> Dependent.const (fun _ _ => True)
              ==> Tensor.eqfR
              ==> Tensor.eqfR
              ==> Tensor.eqfR
@@ -382,8 +392,8 @@ Module HookedTransformer.
           (@masked_attn_scores r batch pos n_heads d_model d_head n_ctx use_split_qkv_input).
     Proof. cbv [masked_attn_scores]; repeat first [ t_step | apply apply_causal_mask_Proper_dep | apply attn_scores_Proper_dep ]. Qed.
 
-    #[export] Instance masked_attn_scores_Proper {r batch pos n_heads d_model d_head n_ctx use_split_qkv_input A sqrtA coerZ addA zeroA mulA divA W_Q W_K b_Q b_K}
-      : Proper (Tensor.eqf ==> Tensor.eqf ==> Tensor.eqf) (@masked_attn_scores r batch pos n_heads d_model d_head n_ctx use_split_qkv_input A sqrtA coerZ addA zeroA mulA divA W_Q W_K b_Q b_K).
+    #[export] Instance masked_attn_scores_Proper {r batch pos n_heads d_model d_head n_ctx use_split_qkv_input A sqrtA coerZ addA zeroA mulA divA use_checkpoint W_Q W_K b_Q b_K}
+      : Proper (Tensor.eqf ==> Tensor.eqf ==> Tensor.eqf) (@masked_attn_scores r batch pos n_heads d_model d_head n_ctx use_split_qkv_input A sqrtA coerZ addA zeroA mulA divA use_checkpoint W_Q W_K b_Q b_K).
     Proof. apply masked_attn_scores_Proper_dep; repeat intro; subst; reflexivity. Qed.
 
     #[export] Instance pattern_Proper_dep {r batch pos n_heads d_model d_head n_ctx use_split_qkv_input}
@@ -395,6 +405,7 @@ Module HookedTransformer.
              ==> (Dependent.idR ==> Dependent.idR ==> Dependent.idR)
              ==> (Dependent.idR ==> Dependent.idR ==> Dependent.idR)
              ==> (Dependent.idR ==> Dependent.idR)
+             ==> Dependent.const (fun _ _ => True)
              ==> Tensor.eqfR
              ==> Tensor.eqfR
              ==> Tensor.eqfR
@@ -405,8 +416,8 @@ Module HookedTransformer.
           (@pattern r batch pos n_heads d_model d_head n_ctx use_split_qkv_input).
     Proof. cbv [pattern]; repeat first [ t_step | apply masked_attn_scores_Proper_dep ]. Qed.
 
-    #[export] Instance pattern_Proper {r batch pos n_heads d_model d_head n_ctx use_split_qkv_input A sqrtA coerZ addA zeroA mulA divA expA W_Q W_K b_Q b_K}
-      : Proper (Tensor.eqf ==> Tensor.eqf ==> Tensor.eqf) (@pattern r batch pos n_heads d_model d_head n_ctx use_split_qkv_input A sqrtA coerZ addA zeroA mulA divA expA W_Q W_K b_Q b_K).
+    #[export] Instance pattern_Proper {r batch pos n_heads d_model d_head n_ctx use_split_qkv_input A sqrtA coerZ addA zeroA mulA divA expA use_checkpoint W_Q W_K b_Q b_K}
+      : Proper (Tensor.eqf ==> Tensor.eqf ==> Tensor.eqf) (@pattern r batch pos n_heads d_model d_head n_ctx use_split_qkv_input A sqrtA coerZ addA zeroA mulA divA expA use_checkpoint W_Q W_K b_Q b_K).
     Proof. apply pattern_Proper_dep; repeat intro; subst; reflexivity. Qed.
 
     #[export] Instance z_Proper_dep {r batch pos n_heads d_model d_head n_ctx use_split_qkv_input}
@@ -418,6 +429,7 @@ Module HookedTransformer.
              ==> (Dependent.idR ==> Dependent.idR ==> Dependent.idR)
              ==> (Dependent.idR ==> Dependent.idR ==> Dependent.idR)
              ==> (Dependent.idR ==> Dependent.idR)
+             ==> Dependent.const (fun _ _ => True)
              ==> Tensor.eqfR
              ==> Tensor.eqfR
              ==> Tensor.eqfR
@@ -429,11 +441,11 @@ Module HookedTransformer.
              ==> Tensor.eqfR
              ==> Tensor.eqfR)
           (@z r batch pos n_heads d_model d_head n_ctx use_split_qkv_input).
-    Proof. cbv [z]; repeat first [ t_step | apply v_Proper_dep | apply pattern_Proper_dep ]. Qed.
+    Proof. cbv [z]; repeat first [ t_step | apply v_Proper_dep | apply pattern_Proper_dep | apply einsum_input_Proper_dep | apply masked_attn_scores_Proper_dep ]. Qed.
 
-    #[export] Instance z_Proper {r batch pos n_heads d_model d_head n_ctx use_split_qkv_input A sqrtA coerZ addA zeroA mulA divA expA W_Q W_K W_V b_Q b_K b_V}
+    #[export] Instance z_Proper {r batch pos n_heads d_model d_head n_ctx use_split_qkv_input A sqrtA coerZ addA zeroA mulA divA expA use_checkpoint W_Q W_K W_V b_Q b_K b_V}
       : Proper (Tensor.eqf ==> Tensor.eqf ==> Tensor.eqf ==> Tensor.eqf)
-          (@z r batch pos n_heads d_model d_head n_ctx use_split_qkv_input A sqrtA coerZ addA zeroA mulA divA expA W_Q W_K W_V b_Q b_K b_V).
+          (@z r batch pos n_heads d_model d_head n_ctx use_split_qkv_input A sqrtA coerZ addA zeroA mulA divA expA use_checkpoint W_Q W_K W_V b_Q b_K b_V).
     Proof. apply z_Proper_dep; repeat intro; subst; reflexivity. Qed.
 
     #[export] Instance attn_out_Proper_dep {r batch pos n_heads d_model d_head n_ctx use_split_qkv_input}
@@ -445,6 +457,7 @@ Module HookedTransformer.
              ==> (Dependent.idR ==> Dependent.idR ==> Dependent.idR)
              ==> (Dependent.idR ==> Dependent.idR ==> Dependent.idR)
              ==> (Dependent.idR ==> Dependent.idR)
+             ==> Dependent.const (fun _ _ => True)
              ==> Tensor.eqfR
              ==> Tensor.eqfR
              ==> Tensor.eqfR
@@ -460,9 +473,9 @@ Module HookedTransformer.
           (@attn_out r batch pos n_heads d_model d_head n_ctx use_split_qkv_input).
     Proof. cbv [attn_out]; repeat first [ t_step | apply z_Proper_dep ]. Qed.
 
-    #[export] Instance attn_out_Proper {r batch pos n_heads d_model d_head n_ctx use_split_qkv_input A sqrtA coerZ addA zeroA mulA divA expA W_Q W_K W_V W_O b_Q b_K b_V b_O}
+    #[export] Instance attn_out_Proper {r batch pos n_heads d_model d_head n_ctx use_split_qkv_input A sqrtA coerZ addA zeroA mulA divA expA use_checkpoint W_Q W_K W_V W_O b_Q b_K b_V b_O}
       : Proper (Tensor.eqf ==> Tensor.eqf ==> Tensor.eqf ==> Tensor.eqf)
-          (@attn_out r batch pos n_heads d_model d_head n_ctx use_split_qkv_input A sqrtA coerZ addA zeroA mulA divA expA W_Q W_K W_V W_O b_Q b_K b_V b_O).
+          (@attn_out r batch pos n_heads d_model d_head n_ctx use_split_qkv_input A sqrtA coerZ addA zeroA mulA divA expA use_checkpoint W_Q W_K W_V W_O b_Q b_K b_V b_O).
     Proof. apply attn_out_Proper_dep; repeat intro; subst; reflexivity. Qed.
   End Attention.
   Export (hints) Attention.
@@ -508,6 +521,7 @@ Module HookedTransformer.
              ==> (Dependent.idR ==> Dependent.idR ==> Dependent.idR)
              ==> (Dependent.idR ==> Dependent.idR ==> Dependent.idR)
              ==> (Dependent.idR ==> Dependent.idR)
+             ==> Dependent.const (fun _ _ => True)
              ==> Dependent.idR
              ==> match normalization_type return Dependent.relation (fun A => match normalization_type with Some LN => _ | None => _ end) with
              | Some LN => Tensor.eqfR (s:=[d_model])
@@ -522,8 +536,8 @@ Module HookedTransformer.
           (@ln1 r batch pos n_heads d_model use_split_qkv_input normalization_type).
     Proof. cbv [ln1]; repeat first [ t_step | apply LayerNorm.forward_Proper_dep ]. Qed.
 
-    #[export] Instance ln1_Proper {r batch pos n_heads d_model use_split_kqv_input normalization_type A zeroA coerZ addA subA mulA divA sqrtA eps ln1_w ln1_b}
-      : Proper (Tensor.eqf ==> Tensor.eqf) (@ln1 r batch pos n_heads d_model use_split_kqv_input normalization_type A zeroA coerZ addA subA mulA divA sqrtA eps ln1_w ln1_b).
+    #[export] Instance ln1_Proper {r batch pos n_heads d_model use_split_kqv_input normalization_type A zeroA coerZ addA subA mulA divA sqrtA eps use_checkpoint ln1_w ln1_b}
+      : Proper (Tensor.eqf ==> Tensor.eqf) (@ln1 r batch pos n_heads d_model use_split_kqv_input normalization_type A zeroA coerZ addA subA mulA divA sqrtA eps use_checkpoint ln1_w ln1_b).
     Proof. apply ln1_Proper_dep; repeat intro; subst; break_innermost_match; reflexivity. Qed.
 
     #[export] Instance ln2_Proper_dep {r batch pos n_heads d_model use_split_qkv_input normalization_type}
@@ -535,6 +549,7 @@ Module HookedTransformer.
              ==> (Dependent.idR ==> Dependent.idR ==> Dependent.idR)
              ==> (Dependent.idR ==> Dependent.idR ==> Dependent.idR)
              ==> (Dependent.idR ==> Dependent.idR)
+             ==> Dependent.const (fun _ _ => True)
              ==> Dependent.idR
              ==> match normalization_type return Dependent.relation (fun A => match normalization_type with Some LN => _ | None => _ end) with
              | Some LN => Tensor.eqfR (s:=[d_model])
@@ -549,8 +564,8 @@ Module HookedTransformer.
           (@ln2 r batch pos n_heads d_model use_split_qkv_input normalization_type).
     Proof. cbv [ln2]; repeat first [ t_step | apply LayerNorm.forward_Proper_dep ]. Qed.
 
-    #[export] Instance ln2_Proper {r batch pos n_heads d_model use_split_kqv_input normalization_type A zeroA coerZ addA subA mulA divA sqrtA eps ln2_w ln2_b}
-      : Proper (Tensor.eqf ==> Tensor.eqf) (@ln2 r batch pos n_heads d_model use_split_kqv_input normalization_type A zeroA coerZ addA subA mulA divA sqrtA eps ln2_w ln2_b).
+    #[export] Instance ln2_Proper {r batch pos n_heads d_model use_split_kqv_input normalization_type A zeroA coerZ addA subA mulA divA sqrtA eps use_checkpoint ln2_w ln2_b}
+      : Proper (Tensor.eqf ==> Tensor.eqf) (@ln2 r batch pos n_heads d_model use_split_kqv_input normalization_type A zeroA coerZ addA subA mulA divA sqrtA eps use_checkpoint ln2_w ln2_b).
     Proof. apply ln2_Proper_dep; repeat intro; subst; break_innermost_match; reflexivity. Qed.
 
     #[export] Instance attn_only_out_Proper_dep {r batch pos n_heads d_model d_head n_ctx use_split_qkv_input normalization_type}
@@ -563,6 +578,7 @@ Module HookedTransformer.
              ==> (Dependent.idR ==> Dependent.idR ==> Dependent.idR)
              ==> (Dependent.idR ==> Dependent.idR)
              ==> (Dependent.idR ==> Dependent.idR)
+             ==> Dependent.const (fun _ _ => True)
              ==> Tensor.eqfR
              ==> Tensor.eqfR
              ==> Tensor.eqfR
@@ -590,8 +606,8 @@ Module HookedTransformer.
       all: first [ apply query_input_Proper_dep | apply key_input_Proper_dep | apply value_input_Proper_dep ]; t.
     Qed.
 
-    #[export] Instance attn_only_out_Proper {r batch pos n_heads d_model d_head n_ctx use_split_kqv_input normalization_type A zeroA coerZ addA subA mulA divA sqrtA expA W_Q W_K W_V W_O b_Q b_K b_V b_O eps ln1_w ln1_b}
-      : Proper (Tensor.eqf ==> Tensor.eqf) (@attn_only_out r batch pos n_heads d_model d_head n_ctx use_split_kqv_input normalization_type A zeroA coerZ addA subA mulA divA sqrtA expA W_Q W_K W_V W_O b_Q b_K b_V b_O eps ln1_w ln1_b).
+    #[export] Instance attn_only_out_Proper {r batch pos n_heads d_model d_head n_ctx use_split_kqv_input normalization_type A zeroA coerZ addA subA mulA divA sqrtA expA W_Q W_K W_V W_O b_Q b_K b_V b_O eps use_checkpoint ln1_w ln1_b}
+      : Proper (Tensor.eqf ==> Tensor.eqf) (@attn_only_out r batch pos n_heads d_model d_head n_ctx use_split_kqv_input normalization_type A zeroA coerZ addA subA mulA divA sqrtA expA W_Q W_K W_V W_O b_Q b_K b_V b_O eps use_checkpoint ln1_w ln1_b).
     Proof. apply attn_only_out_Proper_dep; repeat intro; subst; break_innermost_match; reflexivity. Qed.
 
     #[export] Instance attn_masked_attn_scores_Proper_dep {r batch pos n_heads d_model d_head n_ctx use_split_qkv_input normalization_type}
@@ -603,6 +619,7 @@ Module HookedTransformer.
              ==> (Dependent.idR ==> Dependent.idR ==> Dependent.idR)
              ==> (Dependent.idR ==> Dependent.idR ==> Dependent.idR)
              ==> (Dependent.idR ==> Dependent.idR)
+             ==> Dependent.const (fun _ _ => True)
              ==> Tensor.eqfR
              ==> Tensor.eqfR
              ==> Tensor.eqfR
@@ -626,8 +643,8 @@ Module HookedTransformer.
       all: first [ apply query_input_Proper_dep | apply key_input_Proper_dep ]; t.
     Qed.
 
-    #[export] Instance attn_masked_attn_scores_Proper {r batch pos n_heads d_model d_head n_ctx use_split_kqv_input normalization_type A zeroA coerZ addA subA mulA divA sqrtA W_Q W_K b_Q b_K eps ln1_w ln1_b}
-      : Proper (Tensor.eqf ==> Tensor.eqf) (@HookedTransformer.TransformerBlock.attn_masked_attn_scores r batch pos n_heads d_model d_head n_ctx use_split_kqv_input normalization_type A zeroA coerZ addA subA mulA divA sqrtA W_Q W_K b_Q b_K eps ln1_w ln1_b).
+    #[export] Instance attn_masked_attn_scores_Proper {r batch pos n_heads d_model d_head n_ctx use_split_kqv_input normalization_type A zeroA coerZ addA subA mulA divA sqrtA W_Q W_K b_Q b_K eps use_checkpoint ln1_w ln1_b}
+      : Proper (Tensor.eqf ==> Tensor.eqf) (@HookedTransformer.TransformerBlock.attn_masked_attn_scores r batch pos n_heads d_model d_head n_ctx use_split_kqv_input normalization_type A zeroA coerZ addA subA mulA divA sqrtA W_Q W_K b_Q b_K eps use_checkpoint ln1_w ln1_b).
     Proof. apply attn_masked_attn_scores_Proper_dep; repeat intro; subst; break_innermost_match; reflexivity. Qed.
 
     #[export] Instance attn_pattern_Proper_dep {r batch pos n_heads d_model d_head n_ctx use_split_qkv_input normalization_type}
@@ -640,6 +657,7 @@ Module HookedTransformer.
              ==> (Dependent.idR ==> Dependent.idR ==> Dependent.idR)
              ==> (Dependent.idR ==> Dependent.idR)
              ==> (Dependent.idR ==> Dependent.idR)
+             ==> Dependent.const (fun _ _ => True)
              ==> Tensor.eqfR
              ==> Tensor.eqfR
              ==> Tensor.eqfR
@@ -663,8 +681,8 @@ Module HookedTransformer.
       all: first [ apply query_input_Proper_dep | apply key_input_Proper_dep ]; t.
     Qed.
 
-    #[export] Instance attn_pattern_Proper {r batch pos n_heads d_model d_head n_ctx use_split_kqv_input normalization_type A zeroA coerZ addA subA mulA divA sqrtA expA W_Q W_K b_Q b_K eps ln1_w ln1_b}
-      : Proper (Tensor.eqf ==> Tensor.eqf) (@HookedTransformer.TransformerBlock.attn_pattern r batch pos n_heads d_model d_head n_ctx use_split_kqv_input normalization_type A zeroA coerZ addA subA mulA divA sqrtA expA W_Q W_K b_Q b_K eps ln1_w ln1_b).
+    #[export] Instance attn_pattern_Proper {r batch pos n_heads d_model d_head n_ctx use_split_kqv_input normalization_type A zeroA coerZ addA subA mulA divA sqrtA expA W_Q W_K b_Q b_K eps use_checkpoint ln1_w ln1_b}
+      : Proper (Tensor.eqf ==> Tensor.eqf) (@HookedTransformer.TransformerBlock.attn_pattern r batch pos n_heads d_model d_head n_ctx use_split_kqv_input normalization_type A zeroA coerZ addA subA mulA divA sqrtA expA W_Q W_K b_Q b_K eps use_checkpoint ln1_w ln1_b).
     Proof. apply attn_pattern_Proper_dep; repeat intro; subst; break_innermost_match; reflexivity. Qed.
   End TransformerBlock.
   Export (hints) TransformerBlock.
@@ -694,13 +712,14 @@ Module HookedTransformer.
       : Dependent.Proper
           ((Dependent.const eq ==> Dependent.idR)
              ==> (Dependent.idR ==> Dependent.idR ==> Dependent.idR)
+             ==> Dependent.const (fun _ _ => True)
              ==> Tensor.eqfR ==> Tensor.eqfR
              ==> Dependent.const Tensor.eqf ==> Tensor.eqfR)
           (@resid_postembed d_vocab d_model n_ctx r batch pos).
     Proof. cbv [resid_postembed]; t; first [ apply embed_Proper_dep | apply pos_embed_Proper_dep ]; t. Qed.
 
-    #[export] Instance resid_postembed_Proper {d_vocab d_model n_ctx r batch pos A coerZ addA W_E W_pos}
-      : Proper (Tensor.eqf ==> Tensor.eqf) (@resid_postembed d_vocab d_model n_ctx r batch pos A coerZ addA W_E W_pos).
+    #[export] Instance resid_postembed_Proper {d_vocab d_model n_ctx r batch pos A coerZ addA use_checkpoint W_E W_pos}
+      : Proper (Tensor.eqf ==> Tensor.eqf) (@resid_postembed d_vocab d_model n_ctx r batch pos A coerZ addA use_checkpoint W_E W_pos).
     Proof. apply resid_postembed_Proper_dep; repeat intro; subst; reflexivity. Qed.
 
     #[export] Polymorphic Instance blocks_Proper_dep {n_heads d_model d_head n_ctx r batch pos normalization_type}
@@ -713,6 +732,7 @@ Module HookedTransformer.
              ==> (Dependent.idR ==> Dependent.idR ==> Dependent.idR)
              ==> (Dependent.idR ==> Dependent.idR)
              ==> (Dependent.idR ==> Dependent.idR)
+             ==> Dependent.const (fun _ _ => True)
              ==> Dependent.idR
              ==> List.Forall2 ∘ (Tensor.eqfR * Tensor.eqfR
                                  * Tensor.eqfR * Tensor.eqfR
@@ -737,8 +757,8 @@ Module HookedTransformer.
       apply TransformerBlock.attn_only_out_Proper_dep; t.
     Qed.
 
-    #[export] Polymorphic Instance blocks_Proper {n_heads d_model d_head n_ctx r batch pos normalization_type A zeroA coerZ addA subA mulA divA sqrtA expA eps blocks_params}
-      : Proper (List.Forall2 (Tensor.eqf ==> Tensor.eqf))%signature (@blocks n_heads d_model d_head n_ctx r batch pos normalization_type A zeroA coerZ addA subA mulA divA sqrtA expA eps blocks_params).
+    #[export] Polymorphic Instance blocks_Proper {n_heads d_model d_head n_ctx r batch pos normalization_type A zeroA coerZ addA subA mulA divA sqrtA expA eps use_checkpoint blocks_params}
+      : Proper (List.Forall2 (Tensor.eqf ==> Tensor.eqf))%signature (@blocks n_heads d_model d_head n_ctx r batch pos normalization_type A zeroA coerZ addA subA mulA divA sqrtA expA eps use_checkpoint blocks_params).
     Proof. apply blocks_Proper_dep; repeat intro; subst; break_innermost_match; reflexivity. Qed.
 
     #[export] Instance ln_final_Proper_dep {d_model r batch pos normalization_type}
@@ -764,8 +784,8 @@ Module HookedTransformer.
           (@ln_final d_model r batch pos normalization_type).
     Proof. cbv [ln_final]; repeat first [ t_step | apply LayerNorm.forward_Proper_dep ]. Qed.
 
-    #[export] Instance ln_final_Proper {d_model r batch pos normalization_type A zeroA coerZ addA subA mulA divA sqrtA eps ln_final_w ln_final_b}
-      : Proper (Tensor.eqf ==> Tensor.eqf) (@ln_final d_model r batch pos normalization_type A zeroA coerZ addA subA mulA divA sqrtA eps ln_final_w ln_final_b).
+    #[export] Instance ln_final_Proper {d_model r batch pos normalization_type A zeroA coerZ addA subA mulA divA sqrtA eps use_checkpoint ln_final_w ln_final_b}
+      : Proper (Tensor.eqf ==> Tensor.eqf) (@ln_final d_model r batch pos normalization_type A zeroA coerZ addA subA mulA divA sqrtA eps use_checkpoint ln_final_w ln_final_b).
     Proof. apply ln_final_Proper_dep; repeat intro; subst; break_innermost_match; reflexivity. Qed.
 
     #[export] Instance unembed_Proper_dep {d_vocab_out d_model r batch pos}
@@ -831,9 +851,9 @@ Module HookedTransformer.
       apply TransformerBlock.attn_only_out_Proper_dep; t.
     Qed.
 
-    #[export] Instance blocks_cps_Proper {n_heads d_model d_head n_ctx r batch pos normalization_type A zeroA coerZ addA subA mulA divA sqrtA expA eps blocks_params T R}
+    #[export] Instance blocks_cps_Proper {n_heads d_model d_head n_ctx r batch pos normalization_type A zeroA coerZ addA subA mulA divA sqrtA expA eps use_checkpoint blocks_params T R}
       : Proper (eq ==> Tensor.eqf ==> (Tensor.eqf ==> R) ==> R)
-          (@blocks_cps n_heads d_model d_head n_ctx r batch pos normalization_type A zeroA coerZ addA subA mulA divA sqrtA expA eps blocks_params T).
+          (@blocks_cps n_heads d_model d_head n_ctx r batch pos normalization_type A zeroA coerZ addA subA mulA divA sqrtA expA eps use_checkpoint blocks_params T).
     Proof. apply blocks_cps_Proper_dep; repeat intro; subst; break_innermost_match; reflexivity. Qed.
 
     #[export] Instance logits_Proper_dep {d_vocab d_vocab_out n_heads d_model d_head n_ctx r batch pos normalization_type}
@@ -886,9 +906,9 @@ Module HookedTransformer.
       all: first [ apply resid_postembed_Proper_dep | apply embed_Proper_dep | apply pos_embed_Proper_dep | apply ln_final_Proper_dep | apply unembed_Proper_dep ]; t.
     Qed.
 
-    #[export] Instance logits_Proper {d_vocab d_vocab_out n_heads d_model d_head n_ctx r batch pos normalization_type A zeroA coerZ addA subA mulA divA sqrtA expA eps W_E W_pos blocks_params ln_final_w ln_final_b W_U b_U}
+    #[export] Instance logits_Proper {d_vocab d_vocab_out n_heads d_model d_head n_ctx r batch pos normalization_type A zeroA coerZ addA subA mulA divA sqrtA expA eps use_checkpoint W_E W_pos blocks_params ln_final_w ln_final_b W_U b_U}
       : Proper (Tensor.eqf ==> Tensor.eqf)
-          (@logits d_vocab d_vocab_out n_heads d_model d_head n_ctx r batch pos normalization_type A zeroA coerZ addA subA mulA divA sqrtA expA eps W_E W_pos blocks_params ln_final_w ln_final_b W_U b_U).
+          (@logits d_vocab d_vocab_out n_heads d_model d_head n_ctx r batch pos normalization_type A zeroA coerZ addA subA mulA divA sqrtA expA eps use_checkpoint W_E W_pos blocks_params ln_final_w ln_final_b W_U b_U).
     Proof. apply logits_Proper_dep; repeat intro; subst; break_innermost_match; reflexivity. Qed.
 
     #[export] Instance forward_Proper_dep {d_vocab d_vocab_out n_heads d_model d_head n_ctx r batch pos normalization_type}
@@ -931,9 +951,9 @@ Module HookedTransformer.
           (@forward d_vocab d_vocab_out n_heads d_model d_head n_ctx r batch pos normalization_type)
       := _.
 
-    #[export] Instance forward_Proper {d_vocab d_vocab_out n_heads d_model d_head n_ctx r batch pos normalization_type A zeroA coerZ addA subA mulA divA sqrtA expA eps W_E W_pos blocks_params ln_final_w ln_final_b W_U b_U}
+    #[export] Instance forward_Proper {d_vocab d_vocab_out n_heads d_model d_head n_ctx r batch pos normalization_type A zeroA coerZ addA subA mulA divA sqrtA expA eps use_checkpoint W_E W_pos blocks_params ln_final_w ln_final_b W_U b_U}
       : Proper (Tensor.eqf ==> Tensor.eqf)
-          (@forward d_vocab d_vocab_out n_heads d_model d_head n_ctx r batch pos normalization_type A zeroA coerZ addA subA mulA divA sqrtA expA eps W_E W_pos blocks_params ln_final_w ln_final_b W_U b_U)
+          (@forward d_vocab d_vocab_out n_heads d_model d_head n_ctx r batch pos normalization_type A zeroA coerZ addA subA mulA divA sqrtA expA eps use_checkpoint W_E W_pos blocks_params ln_final_w ln_final_b W_U b_U)
       := _.
 
     #[export] Instance blocks_attn_masked_attn_scores_Proper_dep {n_heads d_model d_head n_ctx r batch pos normalization_type}
@@ -969,9 +989,9 @@ Module HookedTransformer.
       apply TransformerBlock.attn_masked_attn_scores_Proper_dep; t.
     Qed.
 
-    #[export] Instance blocks_attn_masked_attn_scores_Proper {n_heads d_model d_head n_ctx r batch pos normalization_type A zeroA coerZ addA subA mulA divA sqrtA eps blocks_params}
+    #[export] Instance blocks_attn_masked_attn_scores_Proper {n_heads d_model d_head n_ctx r batch pos normalization_type A zeroA coerZ addA subA mulA divA sqrtA eps use_checkpoint blocks_params}
       : Proper (List.Forall2 (Tensor.eqf ==> Tensor.eqf))%signature
-          (@HookedTransformer.HookedTransformer.blocks_attn_masked_attn_scores n_heads d_model d_head n_ctx r batch pos normalization_type A zeroA coerZ addA subA mulA divA sqrtA eps blocks_params).
+          (@HookedTransformer.HookedTransformer.blocks_attn_masked_attn_scores n_heads d_model d_head n_ctx r batch pos normalization_type A zeroA coerZ addA subA mulA divA sqrtA eps use_checkpoint blocks_params).
     Proof. apply blocks_attn_masked_attn_scores_Proper_dep; repeat intro; subst; break_innermost_match; reflexivity. Qed.
 
     #[export] Instance blocks_attn_pattern_Proper_dep {n_heads d_model d_head n_ctx r batch pos normalization_type}
@@ -1008,9 +1028,9 @@ Module HookedTransformer.
       apply TransformerBlock.attn_pattern_Proper_dep; t.
     Qed.
 
-    #[export] Instance blocks_attn_pattern_Proper {n_heads d_model d_head n_ctx r batch pos normalization_type A zeroA coerZ addA subA mulA divA sqrtA expA eps blocks_params}
+    #[export] Instance blocks_attn_pattern_Proper {n_heads d_model d_head n_ctx r batch pos normalization_type A zeroA coerZ addA subA mulA divA sqrtA expA eps use_checkpoint blocks_params}
       : Proper (List.Forall2 (Tensor.eqf ==> Tensor.eqf))%signature
-          (@HookedTransformer.HookedTransformer.blocks_attn_pattern n_heads d_model d_head n_ctx r batch pos normalization_type A zeroA coerZ addA subA mulA divA sqrtA expA eps blocks_params).
+          (@HookedTransformer.HookedTransformer.blocks_attn_pattern n_heads d_model d_head n_ctx r batch pos normalization_type A zeroA coerZ addA subA mulA divA sqrtA expA eps use_checkpoint blocks_params).
     Proof. apply blocks_attn_pattern_Proper_dep; repeat intro; subst; break_innermost_match; reflexivity. Qed.
 
     #[export] Instance masked_attn_scores_Proper_dep {d_vocab n_heads d_model d_head n_ctx r batch pos normalization_type}
@@ -1068,9 +1088,9 @@ Module HookedTransformer.
       all: first [ apply resid_postembed_Proper_dep | apply embed_Proper_dep | apply pos_embed_Proper_dep | apply ln_final_Proper_dep | apply unembed_Proper_dep ]; t.
     Qed.
 
-    #[export] Instance masked_attn_scores_Proper {d_vocab n_heads d_model d_head n_ctx r batch pos normalization_type A zeroA coerZ addA subA mulA divA sqrtA expA eps W_E W_pos blocks_params}
+    #[export] Instance masked_attn_scores_Proper {d_vocab n_heads d_model d_head n_ctx r batch pos normalization_type A zeroA coerZ addA subA mulA divA sqrtA expA eps use_checkpoint W_E W_pos blocks_params}
       : Proper (eq ==> Tensor.eqf ==> option_eq Tensor.eqf)
-          (@HookedTransformer.HookedTransformer.masked_attn_scores d_vocab n_heads d_model d_head n_ctx r batch pos normalization_type A zeroA coerZ addA subA mulA divA sqrtA expA eps W_E W_pos blocks_params).
+          (@HookedTransformer.HookedTransformer.masked_attn_scores d_vocab n_heads d_model d_head n_ctx r batch pos normalization_type A zeroA coerZ addA subA mulA divA sqrtA expA eps use_checkpoint W_E W_pos blocks_params).
     Proof. apply masked_attn_scores_Proper_dep; repeat intro; subst; break_innermost_match; reflexivity. Qed.
 
     #[export] Instance attn_pattern_Proper_dep {d_vocab n_heads d_model d_head n_ctx r batch pos normalization_type}
@@ -1127,9 +1147,9 @@ Module HookedTransformer.
       all: first [ apply resid_postembed_Proper_dep | apply embed_Proper_dep | apply pos_embed_Proper_dep | apply ln_final_Proper_dep | apply unembed_Proper_dep ]; t.
     Qed.
 
-    #[export] Instance attn_pattern_Proper {d_vocab n_heads d_model d_head n_ctx r batch pos normalization_type A zeroA coerZ addA subA mulA divA sqrtA expA eps W_E W_pos blocks_params}
+    #[export] Instance attn_pattern_Proper {d_vocab n_heads d_model d_head n_ctx r batch pos normalization_type A zeroA coerZ addA subA mulA divA sqrtA expA eps use_checkpoint W_E W_pos blocks_params}
       : Proper (eq ==> Tensor.eqf ==> option_eq Tensor.eqf)
-          (@HookedTransformer.HookedTransformer.attn_pattern d_vocab n_heads d_model d_head n_ctx r batch pos normalization_type A zeroA coerZ addA subA mulA divA sqrtA expA eps W_E W_pos blocks_params).
+          (@HookedTransformer.HookedTransformer.attn_pattern d_vocab n_heads d_model d_head n_ctx r batch pos normalization_type A zeroA coerZ addA subA mulA divA sqrtA expA eps use_checkpoint W_E W_pos blocks_params).
     Proof. apply attn_pattern_Proper_dep; repeat intro; subst; break_innermost_match; reflexivity. Qed.
   End HookedTransformer.
   Export (hints) HookedTransformer.
