theories/Util/Default.v
@@ -4,6 +4,7 @@ Definition with_default (name : string) {A} (x : A) := A.
 #[global] Arguments with_default _ {_} _, _ _ _.
 Existing Class with_default.
 #[global] Typeclasses Opaque with_default.
+#[global] Hint Opaque with_default : typeclass_instances.
 Ltac fill_default _ :=
   lazymatch goal with
   | [ |- @with_default ?name ?A ?x ]
@@ -13,4 +14,7 @@ Ltac fill_default _ :=
        end
   end.
 #[global] Hint Extern 0 (with_default _ _) => fill_default () : typeclass_instances.
-#[global] Hint Unfold with_default : typeclass_instances.
+#[global] Hint Extern 0 => lazymatch goal with
+                           | [ |- with_default _ _ ] => fail
+                           | _ => progress unfold with_default
+                           end : typeclass_instances.
